Update Goal Normalization

Grounding_Pipeline.thy
@@ -25,54 +25,54 @@ lemma detyped_valid_iff_compact:
         restrict_classical_problem_axioms.intro wf_ast_classical_problem.intro
   by auto
 
-thm ast_problem.degoal_prob_sel
+thm ast_classical_problem.degoal_prob_sel
 lemma degoal_prob_wf_compact:
-  "wf_problem \<Longrightarrow> ast_problem.wf_problem (degoal_prob)"
-  using wf_ast_problem3.degoal_prob_wf
-  using wf_ast_problem3_def wf_ast_problem.intro by simp
+  "wf_classical_problem \<Longrightarrow> ast_classical_problem.wf_classical_problem (degoal_prob)"
+  using wf_ast_classical_problem3.degoal_prob_wf
+  using wf_ast_classical_problem3_def wf_ast_classical_problem.intro by simp
 lemma degoal_plan_restore_compact:
-  "wf_problem \<Longrightarrow> ast_problem.valid_plan degoal_prob \<pi>s \<Longrightarrow> valid_plan (restore_plan_degoal \<pi>s)"
-  using wf_ast_problem3.valid_plan_left
-  using wf_ast_problem3_def wf_ast_problem.intro by simp
+  "wf_classical_problem \<Longrightarrow> ast_classical_problem.valid_classical_plan2 degoal_prob \<pi>s \<Longrightarrow> valid_classical_plan2 (restore_plan_degoal \<pi>s)"
+  using wf_ast_classical_problem3.valid_classical_plan2_left
+  using wf_ast_classical_problem3_def wf_ast_classical_problem.intro by simp
 lemma degoaled_valid_iff_compact:
-  "wf_problem \<Longrightarrow> (\<exists>\<pi>s. valid_plan \<pi>s) = (\<exists>\<pi>s'. ast_problem.valid_plan degoal_prob \<pi>s')"
-  using wf_ast_problem3.degoaled_valid_iff
-  using wf_ast_problem3_def wf_ast_problem.intro by simp
+  "wf_classical_problem \<Longrightarrow> (\<exists>\<pi>s. valid_classical_plan2 \<pi>s) = (\<exists>\<pi>s'. ast_classical_problem.valid_classical_plan2 degoal_prob \<pi>s')"
+  using wf_ast_classical_problem3.degoaled_valid_iff
+  using wf_ast_classical_problem3_def wf_ast_classical_problem.intro by simp
 
-thm ast_problem.split_prob_sel
-thm ast_problem4.prec_normed_dom
+thm ast_classical_problem.split_prob_sel
+thm ast_classical_problem4.prec_normed_dom
 lemma split_prob_wf_compact:
-  "wf_problem \<Longrightarrow> ast_problem.wf_problem (split_prob)"
-  using wf_ast_problem4.split_prob_wf
-  using wf_ast_problem4_def wf_ast_problem.intro by simp
+  "wf_classical_problem \<Longrightarrow> ast_classical_problem.wf_classical_problem (split_prob)"
+  using wf_ast_classical_problem4.split_prob_wf
+  using wf_ast_classical_problem4_def wf_ast_classical_problem.intro by simp
 lemma split_valid_iff_compact:
-  "wf_problem \<Longrightarrow> (\<exists>\<pi>s. valid_plan \<pi>s) = (\<exists>\<pi>s'. ast_problem.valid_plan split_prob \<pi>s')"
-  using wf_ast_problem4.split_valid_iff
-  using wf_ast_problem4_def wf_ast_problem.intro by simp
+  "wf_classical_problem \<Longrightarrow> (\<exists>\<pi>s. valid_classical_plan \<pi>s) = (\<exists>\<pi>s'. ast_classical_problem.valid_classical_plan split_prob \<pi>s')"
+  using wf_ast_classical_problem4.split_valid_iff
+  using wf_ast_classical_problem4_def wf_ast_classical_problem.intro by simp
 lemma restore_plan_split_valid_compact:
-  "wf_problem \<Longrightarrow> ast_problem.valid_plan split_prob \<pi>s \<Longrightarrow> valid_plan (restore_plan_split \<pi>s)"
-  using wf_ast_problem4.restore_plan_split_valid
-  using wf_ast_problem4_def wf_ast_problem.intro by simp
+  "wf_classical_problem \<Longrightarrow> ast_classical_problem.valid_classical_plan split_prob \<pi>s \<Longrightarrow> valid_classical_plan (restore_plan_split \<pi>s)"
+  using wf_ast_classical_problem4.restore_plan_split_valid
+  using wf_ast_classical_problem4_def wf_ast_classical_problem.intro by simp
 
 lemma relax_wf_relaxed_compact:
-  "wf_problem \<Longrightarrow> normalized_prob \<Longrightarrow>
-    ast_problem.relaxed_prob relax_prob \<and> ast_problem.wf_problem relax_prob"
+  "wf_classical_problem \<Longrightarrow> normalized_prob \<Longrightarrow>
+    ast_classical_problem.relaxed_prob relax_prob \<and> ast_classical_problem.wf_classical_problem relax_prob"
   using normalized_problem_rx.relax_relaxes normalized_problem_rx.relax_wf
   unfolding normalized_problem_rx_def normalized_problem_def' by simp
 lemma relax_normed_compact:
-  "wf_problem \<Longrightarrow> normalized_prob \<Longrightarrow>
-    ast_problem.normalized_prob relax_prob"
+  "wf_classical_problem \<Longrightarrow> normalized_prob \<Longrightarrow>
+    ast_classical_problem.normalized_prob relax_prob"
   using normalized_problem_rx.relax_normed
   unfolding normalized_problem_rx_def normalized_problem_def' by simp
 lemma relax_achievables_compact:
-  "wf_problem \<Longrightarrow> normalized_prob \<Longrightarrow>
-    {a. achievable a} \<subseteq> {a. ast_problem.achievable relax_prob a}"
+  "wf_classical_problem \<Longrightarrow> normalized_prob \<Longrightarrow>
+    {a. achievable a} \<subseteq> {a. ast_classical_problem.achievable relax_prob a}"
   using normalized_problem_rx.relax_achievables
   unfolding normalized_problem_rx_def normalized_problem_def'
   by simp
 lemma relax_applicables_compact:
-  "wf_problem \<Longrightarrow> normalized_prob \<Longrightarrow>
-    {\<pi>. applicable \<pi>} \<subseteq> {\<pi>. ast_problem.applicable relax_prob \<pi>}"
+  "wf_classical_problem \<Longrightarrow> normalized_prob \<Longrightarrow>
+    {\<pi>. applicable \<pi>} \<subseteq> {\<pi>. ast_classical_problem.applicable relax_prob \<pi>}"
   using normalized_problem_rx.relax_applicables
   unfolding normalized_problem_rx_def normalized_problem_def'    
   by simp
@@ -85,17 +85,17 @@ thm grounder.ground_prob_grounded
 thm wf_grounder.ground_prob_wf
 lemma (in wf_grounder) ground_prob_normed:
   assumes "normalized_prob"
-  shows "ast_problem.normalized_prob ground_prob"
+  shows "ast_classical_problem.normalized_prob ground_prob"
   sorry
-thm wf_grounder.valid_plan_iff
-thm wf_grounder.valid_plan_left
+thm wf_grounder.valid_classical_plan_iff
+thm wf_grounder.valid_classical_plan_left
 
 
 lemma wf_as_strips_compact:
-  "wf_problem \<Longrightarrow> grounded_prob \<Longrightarrow> normalized_prob \<Longrightarrow> is_valid_problem_strips as_strips"
+  "wf_classical_problem \<Longrightarrow> grounded_prob \<Longrightarrow> normalized_prob \<Longrightarrow> is_valid_problem_strips as_strips"
   using grounded_normalized_problem.wf_as_strips
   unfolding grounded_normalized_problem_def grounded_normalized_problem_axioms_def
-  unfolding grounded_problem_def grounded_problem_axioms_def wf_ast_problem_def
+  unfolding grounded_problem_def grounded_problem_axioms_def wf_ast_classical_problem_def
   unfolding normalized_prob_def by blast
   
 
@@ -103,24 +103,24 @@ end
 
 subsection \<open> Normalization correctness \<close>
 
-context ast_problem begin
+context ast_classical_problem begin
 
-definition "P\<^sub>N \<equiv> ast_problem.split_prob (ast_problem.degoal_prob detype_prob)"
+definition "P\<^sub>N \<equiv> ast_classical_problem.split_prob (ast_classical_problem.degoal_prob detype_prob)"
 
 definition "reconstruct_plan_norm \<pi>s \<equiv>
   ast_domain.restore_plan_degoal detype_dom
-    (ast_domain.restore_plan_split (ast_problem.degoal_dom detype_prob) \<pi>s)"
+    (ast_domain.restore_plan_split (ast_classical_problem.degoal_dom detype_prob) \<pi>s)"
 
 text \<open> goal and precondition normalization preserve type normalization \<close>
 lemma goal_norm_preserves_typeless:
-  "typeless_prob \<Longrightarrow> ast_problem.typeless_prob (degoal_prob)"
-  unfolding ast_problem.typeless_prob_def ast_domain.typeless_dom_def
+  "typeless_prob \<Longrightarrow> ast_classical_problem.typeless_prob (degoal_prob)"
+  unfolding ast_classical_problem.typeless_prob_def ast_domain.typeless_dom_def
     degoal_prob_sel degoal_dom_sel
   unfolding goal_pred_decl_def goal_ac_def by auto
 
 lemma prec_norm_preserves_typeless:
-  "typeless_prob \<Longrightarrow> ast_problem.typeless_prob (split_prob)"
-  unfolding ast_problem.typeless_prob_def ast_domain.typeless_dom_def
+  "typeless_prob \<Longrightarrow> ast_classical_problem.typeless_prob (split_prob)"
+  unfolding ast_classical_problem.typeless_prob_def ast_domain.typeless_dom_def
     split_prob_sel split_dom_sel
   unfolding split_acs_def using split_ac_sel(2) by auto
 
@@ -149,91 +149,91 @@ lemma goal_norm_preserves_prec_norm:
   using map_preserves_isconj assms(2) by auto
 
 theorem normalization_normalizes:
-  "ast_problem.normalized_prob P\<^sub>N"
-  unfolding ast_problem.normalized_prob_def P\<^sub>N_def
-  using ast_problem2.prob_detyped
-  using ast_problem.degoal_prob_sel(4) ast_problem.goal_norm_preserves_typeless
-  using ast_problem.prec_norm_preserves_typeless ast_problem.prec_norm_preserves_goal_conj
-    ast_problem4.prec_normed_dom
-  by (simp add: ast_problem.split_prob_sel(1))
+  "ast_classical_problem.normalized_prob P\<^sub>N"
+  unfolding ast_classical_problem.normalized_prob_def P\<^sub>N_def
+  using ast_classical_problem2.prob_detyped
+  using ast_classical_problem.degoal_prob_sel(4) ast_classical_problem.goal_norm_preserves_typeless
+  using ast_classical_problem.prec_norm_preserves_typeless ast_classical_problem.prec_norm_preserves_goal_conj
+    ast_classical_problem4.prec_normed_dom
+  by (simp add: ast_classical_problem.split_prob_sel(1))
 
 theorem normalization_wf:
-  "restrict_prob \<Longrightarrow> wf_problem \<Longrightarrow> ast_problem.wf_problem P\<^sub>N"
+  "restrict_prob \<Longrightarrow> wf_classical_problem \<Longrightarrow> ast_classical_problem.wf_classical_problem P\<^sub>N"
   unfolding P\<^sub>N_def
-  using detype_prob_wf_compact ast_problem.degoal_prob_wf_compact ast_problem.split_prob_wf_compact
+  using detype_prob_wf_compact ast_classical_problem.degoal_prob_wf_compact ast_classical_problem.split_prob_wf_compact
   by simp
 
 theorem normalization_valid_iff:
-  "restrict_prob \<Longrightarrow> wf_problem \<Longrightarrow>
-    (\<exists>\<pi>s. valid_plan \<pi>s) \<longleftrightarrow> (\<exists>\<pi>s'. ast_problem.valid_plan P\<^sub>N \<pi>s')"
+  "restrict_prob \<Longrightarrow> wf_classical_problem \<Longrightarrow>
+    (\<exists>\<pi>s. valid_classical_plan \<pi>s) \<longleftrightarrow> (\<exists>\<pi>s'. ast_classical_problem.valid_classical_plan P\<^sub>N \<pi>s')"
   unfolding P\<^sub>N_def
-  using detype_prob_wf_compact ast_problem.degoal_prob_wf_compact
-  using detyped_valid_iff_compact ast_problem.degoaled_valid_iff_compact
-    ast_problem.split_valid_iff_compact by simp
+  using detype_prob_wf_compact ast_classical_problem.degoal_prob_wf_compact
+  using detyped_valid_iff_compact ast_classical_problem.degoaled_valid_iff_compact
+    ast_classical_problem.split_valid_iff_compact by simp
 
 theorem normalization_reconstruct:
-  "restrict_prob \<Longrightarrow> wf_problem \<Longrightarrow>
-    ast_problem.valid_plan P\<^sub>N \<pi>s \<Longrightarrow> valid_plan (reconstruct_plan_norm \<pi>s)"
+  "restrict_prob \<Longrightarrow> wf_classical_problem \<Longrightarrow>
+    ast_classical_problem.valid_classical_plan P\<^sub>N \<pi>s \<Longrightarrow> valid_classical_plan (reconstruct_plan_norm \<pi>s)"
   unfolding P\<^sub>N_def reconstruct_plan_norm_def
-  using detype_prob_wf_compact ast_problem.degoal_prob_wf_compact
-  using ast_problem.restore_plan_split_valid_compact ast_problem.degoal_plan_restore_compact
+  using detype_prob_wf_compact ast_classical_problem.degoal_prob_wf_compact
+  using ast_classical_problem.restore_plan_split_valid_compact ast_classical_problem.degoal_plan_restore_compact
     detyped_valid_iff_compact
-  by (metis ast_problem.degoal_prob_sel(1) detype_prob_sel(1))
+  by (metis ast_classical_problem.degoal_prob_sel(1) detype_prob_sel(1))
 
 end
 
 subsection \<open> Relaxation \<close>
 
-context ast_problem begin
+context ast_classical_problem begin
 
-definition "P\<^sub>R \<equiv> ast_problem.relax_prob P\<^sub>N"
+definition "P\<^sub>R \<equiv> ast_classical_problem.relax_prob P\<^sub>N"
 
 lemma relaxation_applicables:
-  assumes "restrict_prob" "wf_problem"
-  shows "{\<pi>. ast_problem.applicable P\<^sub>N \<pi>} \<subseteq> {\<pi>. ast_problem.applicable P\<^sub>R \<pi>}"
+  assumes "restrict_prob" "wf_classical_problem"
+  shows "{\<pi>. ast_classical_problem.applicable P\<^sub>N \<pi>} \<subseteq> {\<pi>. ast_classical_problem.applicable P\<^sub>R \<pi>}"
   unfolding P\<^sub>R_def
-  using assms normalization_normalizes normalization_wf ast_problem.relax_applicables_compact by simp
+  using assms normalization_normalizes normalization_wf ast_classical_problem.relax_applicables_compact by simp
 
 lemma relaxation_achievables:
-  assumes "restrict_prob" "wf_problem"
-  shows "{a. ast_problem.achievable P\<^sub>N a} \<subseteq> {a. ast_problem.achievable P\<^sub>R a}"
+  assumes "restrict_prob" "wf_classical_problem"
+  shows "{a. ast_classical_problem.achievable P\<^sub>N a} \<subseteq> {a. ast_classical_problem.achievable P\<^sub>R a}"
   unfolding P\<^sub>R_def
-  using assms normalization_normalizes normalization_wf ast_problem.relax_achievables_compact by simp
+  using assms normalization_normalizes normalization_wf ast_classical_problem.relax_achievables_compact by simp
 
 lemma relaxation_wf_relaxed_normed:
-  assumes "restrict_prob" "wf_problem"
-  shows "ast_problem.wf_problem P\<^sub>R" "ast_problem.relaxed_prob P\<^sub>R" "ast_problem.normalized_prob P\<^sub>R"
+  assumes "restrict_prob" "wf_classical_problem"
+  shows "ast_classical_problem.wf_classical_problem P\<^sub>R" "ast_classical_problem.relaxed_prob P\<^sub>R" "ast_classical_problem.normalized_prob P\<^sub>R"
   unfolding P\<^sub>R_def
   using assms normalization_normalizes normalization_wf
-  using ast_problem.relax_wf_relaxed_compact ast_problem.relax_normed_compact
+  using ast_classical_problem.relax_wf_relaxed_compact ast_classical_problem.relax_normed_compact
   by blast+
 
 subsection \<open> Reachability Analysis \<close>
 
-abbreviation "all_facts \<equiv> remdups (snd (ast_problem.semi_naive_eval P\<^sub>R))"
-abbreviation "all_pactions \<equiv> fst (ast_problem.semi_naive_eval P\<^sub>R)"
+abbreviation "all_facts \<equiv> remdups (snd (ast_classical_problem.semi_naive_eval P\<^sub>R))"
+abbreviation "all_pactions \<equiv> fst (ast_classical_problem.semi_naive_eval P\<^sub>R)"
 
 
 thm relaxed_problem.found_facts_achievable
 
 lemma all_facts_solved:
-  assumes "restrict_prob" "wf_problem"
-  shows "set all_facts = {f. ast_problem.achievable P\<^sub>R f}"
+  assumes "restrict_prob" "wf_classical_problem"
+  shows "set all_facts = {f. ast_classical_problem.achievable P\<^sub>R f}"
   using assms relaxed_problem.found_facts_achievable
   using relaxation_wf_relaxed_normed[OF assms]
   by (simp add: normalized_problem_def' relaxed_problem.intro relaxed_problem_axioms_def)
 
 lemma wf_grounder_args:
-  assumes "restrict_prob" "wf_problem"
+  assumes "restrict_prob" "wf_classical_problem"
   shows "wf_grounder P\<^sub>N all_facts all_pactions"
   unfolding wf_grounder_def apply (intro conjI)
   using assms normalization_wf apply blast
           apply simp
   using relaxation_achievables[OF assms] all_facts_solved[OF assms] apply argo
   using relaxation_achievables[OF assms] all_facts_solved[OF assms]
-    wf_ast_problem.achievable_wf normalization_wf[OF assms]
-    wf_ast_problem_def
-  apply (metis P\<^sub>R_def assms ast_domain_rx.rx_wf_fmla_atom ast_problem.relax_prob_sel(1) ast_problem_rx.rx_objT mem_Collect_eq relaxation_wf_relaxed_normed(1))
+    wf_ast_classical_problem.achievable_wf normalization_wf[OF assms]
+    wf_ast_classical_problem_def
+  apply (metis P\<^sub>R_def assms ast_domain_rx.rx_wf_fmla_atom ast_classical_problem.relax_prob_sel(1) ast_classical_problem_rx.rx_objT mem_Collect_eq relaxation_wf_relaxed_normed(1))
   sorry
 
 subsection \<open> Grounding \<close>
@@ -243,51 +243,51 @@ definition "reconstruct_plan_ground \<pi>s =
   reconstruct_plan_norm (grounder.restore_ground_plan all_pactions \<pi>s)"
 
 lemma wf_ground_normed_problem:
-  assumes "restrict_prob" "wf_problem"
-  shows "ast_problem.wf_problem P\<^sub>G" "ast_problem.normalized_prob P\<^sub>G"
-    "ast_problem.grounded_prob P\<^sub>G"
+  assumes "restrict_prob" "wf_classical_problem"
+  shows "ast_classical_problem.wf_classical_problem P\<^sub>G" "ast_classical_problem.normalized_prob P\<^sub>G"
+    "ast_classical_problem.grounded_prob P\<^sub>G"
   using assms wf_grounder_args normalization_normalizes
   using wf_grounder.ground_prob_wf wf_grounder.ground_prob_normed
     grounder.ground_prob_grounded
   by (simp_all add: P\<^sub>G_def)
 
 lemma ground_plan_valid_iff:
-  assumes "restrict_prob" "wf_problem"
-  shows "(\<exists>\<pi>s. valid_plan \<pi>s) \<longleftrightarrow> (\<exists>\<pi>s'. ast_problem.valid_plan P\<^sub>G \<pi>s')"
+  assumes "restrict_prob" "wf_classical_problem"
+  shows "(\<exists>\<pi>s. valid_classical_plan \<pi>s) \<longleftrightarrow> (\<exists>\<pi>s'. ast_classical_problem.valid_classical_plan P\<^sub>G \<pi>s')"
   using assms normalization_valid_iff wf_grounder_args
-  using wf_grounder.valid_plan_iff
+  using wf_grounder.valid_classical_plan_iff
   unfolding P\<^sub>G_def by blast
 
 lemma ground_plan_reconstruct:
-  assumes "restrict_prob" "wf_problem"
-  shows "ast_problem.valid_plan P\<^sub>G \<pi>s \<Longrightarrow>
-    valid_plan (reconstruct_plan_ground \<pi>s)"
+  assumes "restrict_prob" "wf_classical_problem"
+  shows "ast_classical_problem.valid_classical_plan P\<^sub>G \<pi>s \<Longrightarrow>
+    valid_classical_plan (reconstruct_plan_ground \<pi>s)"
   using assms normalization_reconstruct wf_grounder_args
-  using wf_grounder.valid_plan_left normalization_reconstruct
+  using wf_grounder.valid_classical_plan_left normalization_reconstruct
   unfolding P\<^sub>G_def reconstruct_plan_ground_def by simp
 
 subsection \<open> Conversion to STRIPS \<close>
-definition "P\<^sub>S \<equiv> ast_problem.as_strips P\<^sub>G"
+definition "P\<^sub>S \<equiv> ast_classical_problem.as_strips P\<^sub>G"
 definition "reconstruct_pipeline_plan ops \<equiv>
-  reconstruct_plan_ground (ast_problem.restore_pddl_plan P\<^sub>G ops)"
+  reconstruct_plan_ground (ast_classical_problem.restore_pddl_plan P\<^sub>G ops)"
 
 lemma wf_as_strips:
-  assumes "restrict_prob" "wf_problem"
+  assumes "restrict_prob" "wf_classical_problem"
   shows "is_valid_problem_strips P\<^sub>S"
-  using assms ast_problem.wf_as_strips_compact
+  using assms ast_classical_problem.wf_as_strips_compact
   using wf_ground_normed_problem
   unfolding P\<^sub>S_def by blast
 
 lemma strips_plan_reconstruct:
-  assumes "restrict_prob" "wf_problem"
+  assumes "restrict_prob" "wf_classical_problem"
   shows "is_serial_solution_for_problem P\<^sub>S ops \<Longrightarrow>
-    valid_plan (reconstruct_pipeline_plan ops)"
+    valid_classical_plan (reconstruct_pipeline_plan ops)"
   oops
 
 lemma strips_plan_iff:
-  assumes "restrict_prob" "wf_problem"
+  assumes "restrict_prob" "wf_classical_problem"
   shows "(\<exists>ops. is_serial_solution_for_problem P\<^sub>S ops) \<longleftrightarrow>
-    (\<exists>\<pi>s. valid_plan \<pi>s)"
+    (\<exists>\<pi>s. valid_classical_plan \<pi>s)"
   oops
 
 end
